hastype_lambda/chap9_deBruijn.v
@@ -1,0 +1,598 @@
+Require Coq.extraction.Extraction.
+Require Import Ascii String Coq.Strings.Byte.
+Require Export ExtrOcamlChar.
+Extract Inductive bool => "bool" ["true" "false"].
+Extract Inductive string => "char list" [ "[]" "(::)" ].
+From Coq Require Import Lists.List.
+Extract Inductive list => "list" [ "[]" "(::)" ].
+Extraction Language OCaml.
+Import ListNotations.
+Require Import std.
+
+
+Inductive ty : Type :=
+| Bool
+|Arrow (ty1 ty2: ty).
+Notation "t1 '|-->' t2" := (Arrow t1 t2) (at level 40).
+
+Inductive term : Type :=
+(*純粋λ計算*)
+| Var (n: nat)
+| Abs (name: string) (typ: ty) (t: term)
+| App (t1 t2: term)
+(*ぶーる*)
+| Tru
+| Fls
+| If (t1 t2 t3: term).
+
+Definition context : Type :=
+  list (string * ty).
+
+Definition eqb_string s1 s2:=
+  String.eqb s1 s2.
+
+Definition addbind (ctx: context) x bind :=
+  (x, bind) :: ctx.
+
+
+Fixpoint getbinding (n : nat) (ctx: context) :=
+  match n with
+  | 0 =>
+    match ctx with
+    | [] => None
+    | (x, t) :: ctx' => Some t
+    end
+  | S n' =>
+    match ctx with
+    | [] => None
+    | x :: ctx' => getbinding n' ctx'
+    end
+  end.
+
+Definition isval t:=
+match t with
+| Tru => true
+| Fls => true
+| Abs _ _ _ => true
+| _ => false
+end.
+
+Inductive N : Type :=
+| P (n: nat)
+| M1.
+
+Fixpoint shift_walk c d t :=
+  match t with
+  | Var x =>
+    if leb c x then
+      match d with
+      | M1 =>
+        Var (x - 1)
+      | P d' =>
+        Var (x + d')
+      end
+    else
+      Var x
+  | Abs t x t1 =>
+    Abs t x (shift_walk (S c) d t1)
+  | App t1 t2 =>
+    App (shift_walk c d t1) (shift_walk c d t2)
+  | If t1 t2 t3 =>
+    If (shift_walk c d t1) (shift_walk c d t2) (shift_walk c d t3)
+  | _ => t
+  end.
+
+Notation shift d t := (shift_walk 0 d t).
+
+Fixpoint sub_walk j s c t :=
+  match t with
+  | Var x =>
+    let jc :=
+        match c with
+        | M1 => (j - 1)
+        | P c' => (j + c')
+        end
+    in
+    if eqb_nat x (jc) then
+      shift c s
+    else
+      Var x
+  | Abs t x t1 =>
+    let sc :=
+        match c with
+        | M1 => P 0
+        | P c' => P (c' + 1)
+        end
+    in
+    Abs t x (sub_walk j s sc t1)
+  | App t1 t2 =>
+    App (sub_walk j s c t1) (sub_walk j s c t2)
+  | If t1 t2 t3 =>
+    If (sub_walk j s c t1) (sub_walk j s c t2) (sub_walk j s c t3)
+  | _ => t
+  end.
+
+Notation sub j s t := (sub_walk j s (P 0) t).
+
+Notation subtop s t := (shift M1 (sub 0 (shift (P 1) s) t)).
+
+Inductive value : term -> Prop :=
+| V_tru : value Tru
+| V_fls : value Fls
+| V_abs :forall typ name t1, value (Abs typ name t1).
+
+
+Reserved Notation " t '-->' t' " (at level 40).
+Inductive step :term -> term -> Prop :=
+| E_IfTrue : forall t2 t3,
+    If Tru t2 t3 --> t2
+| E_IfFalse : forall t2 t3,
+    If Fls t2 t3 --> t3
+| E_If : forall t1 t1' t2 t3,
+    t1 --> t1' ->
+    If t1 t2 t3 --> If t1' t2 t3
+| E_App1 : forall t1 t2 t1',
+    t1 --> t1' ->
+    App t1 t2 --> App t1' t2
+| E_App2 : forall v1 t2 t2',
+    value v1 ->
+    t2 --> t2' ->
+    App v1 t2 --> App v1 t2'
+| E_AppAbs : forall typ str t12 t2,
+    value t2 ->
+    App (Abs typ str t12) t2 --> subtop t2 t12
+
+  where " t '-->' t' " := (step t t').
+
+Fixpoint eqb_ty (T1 T2: ty) : bool :=
+  match (T1, T2) with
+  | (Bool, Bool) => true
+  | (T11 |--> T12, T21 |--> T22) =>
+    andb (eqb_ty T11 T21) (eqb_ty T12 T22)
+  | _ => false
+  end.
+
+Fixpoint inb (ctx: context) (name: string) (T: ty): bool :=
+  match ctx with
+    | [] => false
+    | (n1, b) :: m =>
+      if andb (eqb_string name n1) (eqb_ty T b) then
+        true
+      else inb m name T
+  end.
+
+Reserved Notation "ctx '|-' x '\in' t" (at level 40).
+Inductive has_type : context -> term -> ty -> Prop :=
+| T_True:
+    forall ctx,
+      ctx |- Tru \in Bool
+| T_False:
+    forall ctx,
+      ctx |- Fls \in Bool
+| T_If:
+    forall ctx t1 t2 t3 T',
+      ctx |- t1 \in Bool ->
+      ctx |- t2 \in T' ->
+      ctx |- t3 \in T' ->
+      ctx |- (If t1 t2 t3) \in T'
+| T_Var:
+    forall ctx n1 t,
+      getbinding n1 ctx = Some t ->
+      ctx |- (Var n1) \in t
+| T_Abs:
+    forall ctx x T1 t2 T2,
+      (addbind ctx x T1) |- t2 \in T2 ->
+      ctx |- (Abs x T1 t2) \in (T1 |--> T2)
+| T_App:
+    forall ctx t1 T11 T12 t2,
+      ctx |- t1 \in (T11 |--> T12) ->
+      ctx |- t2 \in T11 ->
+      ctx |- App t1 t2 \in T12
+
+where " ctx '|-' x '\in' t " := (has_type ctx x t).
+
+
+Example type1:
+  [("f"%string, (Bool |--> Bool))] |- App (Var 0) (If Fls Tru Fls) \in Bool.
+Proof.
+  eapply T_App. apply T_Var. reflexivity.
+  apply T_If. apply T_False. apply T_True. apply T_False.
+Qed.
+
+Example type2:
+  [("f"%string, (Bool |--> Bool))] |- (Abs "x" Bool (App (Var 1) (If (Var 0) Fls (Var 0)))) \in (Bool |--> Bool).
+Proof.
+  apply T_Abs. eapply T_App. apply T_Var. reflexivity.
+  apply T_If. apply T_Var. reflexivity. apply T_False. apply T_Var. reflexivity.
+Qed.
+
+Lemma eqb_ty_eq : forall T1 T2,
+    eqb_ty T1 T2 = true <-> T1 = T2.
+Proof.
+  split; intros.
+  generalize dependent T2; induction T1; intros.
+  destruct T2; auto. inversion H.
+  inversion H. destruct T2. inversion H1. apply andb_prop in H1.
+  inversion H1. apply IHT1_1 in H0. apply IHT1_2 in H2. rewrite H0, H2. reflexivity.
+
+  generalize dependent T2; induction T1; intros.
+  destruct T2. reflexivity. inversion H.
+
+  destruct T2; auto. inversion H.
+  simpl. inversion H. rewrite <- H1. rewrite <- H2. apply andb_true_intro.
+  split; auto.
+Qed.
+
+
+Lemma E9_3_2 :  forall n T,
+    not (exists ctx,ctx |- App (Var n) (Var n) \in T).
+Proof.
+  intros; intro. inversion H.
+  inversion H0; subst. inversion H4. inversion H6; subst.
+  rewrite H9 in H3. inversion H3. apply eqb_ty_eq in H2.
+  generalize H2. clear. generalize dependent T.
+  induction T11; intros. inversion H2. inversion H2. apply andb_prop in H0. inversion H0.
+  apply IHT11_1 in H. apply H.
+Qed.
+
+Lemma T9_3_3 : forall t1 ctx T1 T2,
+    ctx |- t1 \in T1 ->
+    ctx |- t1 \in T2 ->
+    T1 = T2.
+Proof.
+  induction t1; intros.
+  -
+    inversion H; inversion H0; subst. rewrite H3 in H7. inversion H7; reflexivity.
+  -
+    inversion H; inversion H0; subst.
+    apply eqb_ty_eq. simpl; apply andb_true_intro; split; auto.
+    clear. induction typ; auto. simpl. apply andb_true_intro. split; auto.
+    apply eqb_ty_eq. apply (IHt1 (addbind ctx name typ) T3 T5); auto.
+  -
+    inversion H; inversion H0; subst.
+    apply IHt1_1 with (T2:= (T0 |--> T2)) in H4; auto.
+    inversion H4; reflexivity.
+  -
+    inversion H; inversion H0; subst; auto.
+  -
+    inversion H; inversion H0; subst; auto.
+  -
+    inversion H; inversion H0; subst; auto.
+    apply (IHt1_2 ctx T1 T2); auto.
+Qed.
+
+Lemma L9_3_4_bool : forall ctx v,
+    value v ->
+    ctx |- v \in Bool ->
+    v = Tru \/ v = Fls.
+Proof.
+  intros. inversion H0; subst. left; auto. right; auto.
+  inversion H. inversion H. inversion H.
+Qed.
+
+Lemma L9_3_4_Abs: forall ctx v T1 T2,
+    value v ->
+    ctx |- v \in (T1 |--> T2) ->
+    exists x t, v = Abs x T1 t.
+Proof.
+  intros. inversion H0; subst; try solve_by_invert.
+  exists x, t2. reflexivity.
+Qed.
+
+Theorem T9_3_5 : forall t T,
+    [] |- t \in T ->
+    value t \/ exists t', t --> t'.
+Proof.
+  induction t; simpl; intros.
+  -
+    inversion H; subst. destruct n; inversion H2.
+  -
+    left; apply V_abs.
+  -
+    right.
+    inversion H; subst.
+    generalize H3; intro. apply IHt1 in H3. destruct H3.
+    apply (L9_3_4_Abs [] t1) in H0; auto. inversion H0. inversion H2.
+    apply IHt2 in H5. inversion H5. rewrite H3.
+    exists (subtop t2 x0). apply E_AppAbs; auto.
+    inversion H4. exists (App t1 x1). apply E_App2; auto.
+    inversion H1. exists (App x t2); apply E_App1; auto.
+  -
+    left. apply V_tru.
+  -
+    left; apply V_fls.
+  -
+    inversion H; subst. right. generalize H4; intros; apply IHt1 in H4.
+    destruct H4. apply (L9_3_4_bool [] t1) in H1; auto. destruct H1; rewrite H1.
+    exists t2; apply E_IfTrue. exists t3; apply E_IfFalse. inversion H1.
+    exists (If x t2 t3); apply E_If; auto.
+Qed.
+
+Notation " x :-> T ;; ctx" := (addbind ctx x T) (at level 50).
+
+Lemma leb_0_T : forall n,
+    leb 0 n = true.
+Proof.
+  induction n; auto.
+Qed.
+
+Lemma shift0_refl : forall t n,
+    shift_walk n (P 0) t = t.
+Proof.
+  induction t; simpl; intros; auto.
+  destruct (leb n0 n). rewrite <- plus_n_O. reflexivity.
+  reflexivity. rewrite IHt. reflexivity.
+  rewrite IHt1. rewrite IHt2. reflexivity.
+  rewrite IHt1. rewrite IHt2. rewrite IHt3. reflexivity.
+Qed.
+
+Lemma shift_m1_p1_refl : forall t n,
+    shift_walk n (M1) (shift_walk n (P 1) t) = t.
+Proof.
+  induction t; intros; simpl; auto.
+  -
+    destruct (leb n0 n) eqn:IH. simpl. apply le_leb in IH. apply PeanoNat.Nat.le_le_succ_r in IH. apply leb_le in IH. rewrite PeanoNat.Nat.add_1_r. rewrite IH. simpl. rewrite PeanoNat.Nat.sub_0_r. reflexivity.
+
+    simpl. rewrite IH. reflexivity.
+  -
+    rewrite IHt. reflexivity.
+  -
+    rewrite IHt2. rewrite IHt1. reflexivity.
+  -
+    rewrite IHt3, IHt2, IHt1.  reflexivity.
+Qed.
+
+Lemma L9_3_8: forall t s x S T ctx,
+    addbind ctx x S |- t \in T ->
+    ctx |- s \in S ->
+    ctx |- subtop s t \in T.
+Proof.
+   induction t; simpl; intros.
+   -
+     rewrite shift0_refl. destruct (eqb_nat n 0) eqn:IH. apply eqb_eq in IH. subst.
+     rewrite shift_m1_p1_refl. inversion H; subst. inversion H3; subst. apply H0.
+     destruct n. inversion IH. simpl. rewrite leb_0_T. inversion H; subst. unfold getbinding in H3. simpl in H3. fold getbinding in H3. apply T_Var. rewrite PeanoNat.Nat.sub_0_r. apply H3.
+   -
+     inversion H; subst. apply T_Abs.
+     admit.
+   -
+     inversion H; subst. apply T_App with T11. eapply IHt1. apply H4. apply H0.
+     eapply IHt2. apply H6. apply H0.
+   -
+     inversion H; subst. apply T_True.
+   -
+     inversion H; subst. apply T_False.
+   -
+     inversion H; subst.
+     apply T_If. eapply IHt1; auto. apply H5. apply H0. eapply IHt2. apply H7. apply H0. eapply IHt3. apply H8. apply H0.
+Abort.
+
+Lemma L9_3_8: forall t s x S T ctx,
+    addbind ctx x S |- t \in T ->
+    ctx |- s \in S ->
+    ctx |- subtop s t \in T.
+Proof.
+  intros. remember (x :-> S ;; ctx) as Gamma; generalize dependent s; induction H; simpl; intros.
+  apply T_True. apply T_False.
+  apply T_If; auto.
+
+  destruct (eqb_nat n1 0) eqn:IH. apply eqb_eq in IH. subst.
+  inversion H; subst. clear H. induction H0; simpl.
+  apply T_True. apply T_False. apply T_If; auto.
+  rewrite leb_0_T.
+
+
+  destruct n1. rewrite shift0_refl. simpl. apply T_Var. apply H.
+  rewrite shift0_refl. simpl. rewrite leb_0_T. apply T_Var. rewrite PeanoNat.Nat.sub_0_r.
+  rewrite PeanoNat.Nat.add_1_r. apply H.
+
+  rewrite shift0_refl. rewrite shift0_refl in IHhas_type. apply T_Abs. rewrite shift_m1_p1_refl. apply H0.
+
+
+  eapply T_App. rewrite shift0_refl.
+  rewrite shift0_refl in IHhas_type1. rewrite shift0_refl in IHhas_type2.
+  apply IHhas_type1. apply IHhas_type2.
+
+
+  simpl. rewrite leb_0_T. destruct n1.
+  inversion IH. inversion H; subst.
+  unfold getbinding in H2. fold getbinding in H2. simpl in H2. simpl.
+  rewrite PeanoNat.Nat.sub_0_r. apply T_Var. apply H2.
+
+  apply T_Abs. subst.
+  admit.
+
+  eapply T_App. apply IHhas_type1; auto. apply IHhas_type2; auto.
+Admitted.
+
+Theorem T9_3_9 : forall t t' T ctx,
+    ctx |- t \in T ->
+    t --> t' ->
+    ctx |- t' \in T.
+Proof.
+  intros. generalize dependent T. induction H0; subst; simpl; intros; auto.
+  -
+    inversion H; subst. apply H6.
+  -
+    inversion H; subst. apply H7.
+  -
+    inversion H; subst. apply IHstep in H5. apply T_If; auto.
+  -
+    inversion H; subst. apply IHstep in H4. apply T_App with T11; auto.
+  -
+    inversion H1; subst. apply IHstep in H7. apply T_App with T11; auto.
+  -
+    inversion H0; subst. clear H0.
+    inversion H4; subst. eapply L9_3_8; eauto.
+Qed.
+
+Fixpoint typeof ctx t : option ty :=
+  match t with
+  | Tru =>
+    (Some Bool)
+  | Fls =>
+    Some Bool
+  | If t1 t2 t3 =>
+    match typeof ctx t1 with
+    | Some Bool =>
+      match typeof ctx t2 with
+      | Some T2 =>
+        match typeof ctx t3 with
+        | Some T3 =>
+          if eqb_ty T2 T3 then
+            Some T2
+          else
+            None
+        | None => None
+        end
+      | None => None
+      end
+    | _ => None
+    end
+  | Var n =>
+    getbinding n ctx
+  | Abs x T1 t1 =>
+    match typeof (x :-> T1 ;; ctx) t1 with
+    | Some T2 =>
+      Some (T1 |--> T2)
+    | None => None
+    end
+  | App t1 t2 =>
+    match typeof ctx t1 with
+    | Some (T11 |--> T12) =>
+      match typeof ctx t2 with
+      | Some T21 =>
+        if eqb_ty T11 T21 then
+          Some T12
+        else
+          None
+      | None => None
+      end
+    | _ => None
+    end
+  end.
+
+Lemma eq_type_refl : forall T,
+    eqb_ty T T = true.
+Proof.
+  induction T; simpl; auto. rewrite IHT1, IHT2; auto.
+Qed.
+
+Lemma typeof_hasType : forall t ctx T,
+    has_type ctx t T <-> typeof ctx t = Some T.
+Proof.
+  split; intros.
+  -
+    induction H; simpl; auto.
+    +
+      rewrite IHhas_type1, IHhas_type2, IHhas_type3. clear.
+      rewrite eq_type_refl; reflexivity.
+    +
+      rewrite IHhas_type. reflexivity.
+    +
+      rewrite IHhas_type2, IHhas_type1. rewrite eq_type_refl; reflexivity.
+  -
+    generalize dependent T. generalize dependent ctx; induction t; intros; simpl; auto.
+    +
+      inversion H; subst; apply T_Var; simpl; auto.
+    +
+      inversion H; subst. destruct (typeof (name :-> typ;; ctx) t) eqn:IH. inversion H1; subst.
+      apply IHt in IH. apply T_Abs. apply IH. inversion H1.
+    +
+      inversion H. destruct (typeof ctx t1) eqn:IH1. destruct (typeof ctx t2) eqn:IH2. apply IHt1 in IH1. apply IHt2 in IH2. destruct t. inversion H1. destruct (eqb_ty t3 t0) eqn:IH3. apply eqb_ty_eq in IH3. subst. inversion H1; subst. eapply T_App; eauto. inversion H1. destruct t. inversion H1. inversion H1. inversion H1.
+    +
+      inversion H. apply T_True.
+    +
+      inversion H. apply T_False.
+    +
+      inversion H. destruct (typeof ctx t1) eqn:IH1. destruct (typeof ctx t2) eqn:IH2. apply IHt1 in IH1. apply IHt2 in IH2. destruct (typeof ctx t3) eqn:IH3. apply IHt3 in IH3. destruct t.
+      destruct (eqb_ty t0 t4) eqn:IH4. apply eqb_ty_eq in IH4. subst. inversion H1; subst. eapply T_If; eauto.
+      inversion H1. inversion H1. destruct t; try solve_by_invert. destruct t; try solve_by_invert. inversion H1.
+Qed.
+
+Fixpoint eval (t: term) :=
+  match t with
+  | If t1 t2 t3 =>
+    match t1 with
+    | Tru => Some t2
+    | Fls => Some t3
+    | _ => match eval t1 with
+          | Some t1' =>
+            Some (If t1' t2 t3)
+          | None => None
+          end
+    end
+  | App t1 t2 =>
+    if isval t1 then
+      if isval t2 then
+        match t1 with
+        | Abs _ _ t12 => Some (subtop t2 t12)
+        | _ => None
+        end
+      else
+        match eval t2 with
+        | Some t2' => Some (App t1 t2')
+        | None => None
+        end
+    else
+      match eval t1 with
+      | Some t1' => Some (App t1' t2)
+      | None => None
+      end
+  | _ => None
+  end.
+
+Lemma isval_no_step : forall t,
+    isval t = true -> not (exists t', t --> t').
+Proof.
+  intros. destruct t; try solve_by_invert; intro;
+  inversion H0; inversion H1.
+Qed.
+
+Lemma isval_value : forall t,
+    value t <-> isval t = true.
+Proof.
+  split; intros; destruct t; try solve_by_invert; auto.
+  apply V_abs. apply V_tru. apply V_fls.
+Qed.
+
+Lemma isval_F : forall t t',
+    eval t = Some t' -> isval t = false.
+Proof.
+  intros. destruct t; try solve_by_invert; auto.
+Qed.
+
+Lemma isval_eval : forall t t',
+    t --> t' ->
+    isval t = false.
+Proof.
+  intros. inversion H; subst; auto.
+Qed.
+
+Lemma eval_step : forall t t',
+    t --> t' <-> eval t = Some t'.
+Proof.
+  split; intros.
+  -
+    induction H; simpl; eauto.
+    +
+      rewrite IHstep. destruct t1; try solve_by_invert; auto.
+    +
+      rewrite IHstep. apply isval_eval in H. rewrite H. reflexivity.
+    +
+      rewrite IHstep. apply isval_eval in H0. rewrite H0. apply isval_value in H. rewrite H.
+      reflexivity.
+    +
+      apply isval_value in H. rewrite H. reflexivity.
+  -
+    generalize dependent t'. induction t; intros; try solve_by_invert; auto; inversion H.
+    +
+      destruct (isval t1) eqn:IH1. destruct (isval t2) eqn:IH2.
+      apply isval_value in IH1. inversion IH1; subst; try solve_by_invert.
+      inversion H1. apply E_AppAbs. apply isval_value; auto.
+      destruct (eval t2). inversion H1. apply E_App2. apply isval_value; auto. apply IHt2; auto.
+      inversion H1.
+      destruct (eval t1) eqn:IHH; try solve_by_invert. inversion H1. apply E_App1. apply IHt1; auto.
+    +
+      destruct (eval t1) eqn:IH; destruct t1; try solve_by_invert; inversion H1; try (apply E_If; apply IHt1; reflexivity). apply E_IfTrue. apply E_IfFalse.
+Qed.
