hastype_lambda/chap9_string.v
@@ -1,0 +1,419 @@
+Require Coq.extraction.Extraction.
+Require Import Ascii String Coq.Strings.Byte.
+Require Export ExtrOcamlChar.
+Extract Inductive bool => "bool" ["true" "false"].
+Extract Inductive string => "char list" [ "[]" "(::)" ].
+From Coq Require Import Lists.List.
+Extract Inductive list => "list" [ "[]" "(::)" ].
+Extraction Language OCaml.
+Import ListNotations.
+Require Import std.
+
+Inductive ty : Type :=
+| Bool
+|Arrow (ty1 ty2: ty).
+Notation "t1 '|-->' t2" := (Arrow t1 t2) (at level 40).
+
+Inductive term : Type :=
+(*純粋λ計算*)
+| var (name: string)
+| abs (name: string) (typ: ty) (t: term)
+| app (t1 t2: term)
+(*ぶーる*)
+| tru
+| fls
+| If (t1 t2 t3: term).
+
+Inductive value : term -> Prop :=
+  | v_abs : forall x T t,
+      value (abs x T t)
+  | v_tru :
+      value tru
+  | v_fls :
+      value fls.
+
+
+Reserved Notation "'[' x ':=' s ']' t" (at level 20).
+
+Fixpoint subst (x : string) (s : term) (t : term) : term :=
+  match t with
+  | var x' =>
+      if String.eqb x x' then s else t
+  | abs x' T t1 =>
+      abs x' T (if String.eqb x x' then t1 else ([x:=s] t1))
+  | app t1 t2 =>
+      app ([x:=s] t1) ([x:=s] t2)
+  | tru =>
+      tru
+  | fls =>
+      fls
+  | If t1 t2 t3 =>
+      If ([x:=s] t1) ([x:=s] t2) ([x:=s] t3)
+  end
+
+where "'[' x ':=' s ']' t" := (subst x s t).
+
+Inductive substi (s : term) (x : string) : term -> term -> Prop :=
+  | s_var1 :
+      substi s x (var x) s
+  | s_var2 : forall str,
+      x <> str ->
+      substi s x (var str) (var str)
+  | s_abs1 : forall T t1,
+      substi s x (abs x T t1) (abs x T t1)
+  | s_abs2 : forall str T t1 t',
+      x <> str ->
+      substi s x t1 t' ->
+      substi s x (abs str T t1) (abs str T t')
+  | s_app : forall t1 t2 t1' t2',
+      substi s x t1 t1' ->
+      substi s x t2 t2' ->
+      substi s x (app t1 t2) (app t1' t2')
+  | s_tru :
+    substi s x tru tru
+  | s_fls :
+    substi s x fls fls
+  | s_if : forall t1 t2 t3 t1' t2' t3',
+      substi s x t1 t1' ->
+      substi s x t2 t2' ->
+      substi s x t3 t3' ->
+      substi s x (If t1 t2 t3) (If t1' t2' t3')
+.
+Theorem substi_correct : forall t s x t',
+  [x:=s]t = t' <-> substi s x t t'.
+Proof.
+  split.
+  -
+    generalize dependent s. generalize dependent t'. induction t; intros; auto.
+    +
+      unfold subst in H. destruct (x =? name)%string eqn:IH1.
+      apply String.eqb_eq in IH1. rewrite IH1. rewrite H. apply s_var1.
+      apply eqb_neq in IH1. rewrite <- H. apply s_var2; auto.
+    +
+      unfold subst in H.
+      destruct (x =? name)%string eqn:IH1. apply String.eqb_eq in IH1. rewrite IH1.
+      rewrite <- H. apply s_abs1.
+      apply eqb_neq in IH1. fold subst in H. rewrite <- H. apply s_abs2; auto.
+    +
+      simpl in H. rewrite <- H. apply s_app; auto.
+    +
+      simpl in H. rewrite <- H. apply s_tru.
+    +
+      simpl in H. rewrite <- H. apply s_fls.
+    +
+      rewrite <- H. simpl. apply s_if; auto.
+  -
+    intros. induction H; simpl; auto.
+    +
+      rewrite eqb_refl. reflexivity.
+    +
+      apply eqb_neq in H. rewrite H. reflexivity.
+    +
+      rewrite eqb_refl. reflexivity.
+    +
+      apply eqb_neq in H. rewrite H. rewrite IHsubsti. reflexivity.
+    +
+      rewrite <- IHsubsti1. rewrite <- IHsubsti2. reflexivity.
+    +
+      rewrite <- IHsubsti2, IHsubsti1, IHsubsti3. reflexivity.
+Qed.
+
+
+Reserved Notation "t1 '-->' t2" (at level 40).
+
+Inductive step : term -> term -> Prop :=
+  | E_AppAbs : forall x T t12 v2,
+         value v2 ->
+         (app (abs x T t12) v2) --> [x:=v2]t12
+  | E_App1 : forall t1 t1' t2,
+         t1 --> t1' ->
+         app t1 t2 --> app t1' t2
+  | E_App2 : forall v1 t2 t2',
+         value v1 ->
+         t2 --> t2' ->
+         app v1 t2 --> app v1 t2'
+  | E_IfTru : forall t1 t2,
+      (If tru t1 t2) --> t1
+  | E_IfFls : forall t1 t2,
+      (If fls t1 t2) --> t2
+  | E_If : forall t1 t1' t2 t3,
+      t1 --> t1' ->
+      (If t1 t2 t3) --> (If t1' t2 t3)
+
+where "t1 '-->' t2" := (step t1 t2).
+
+Reserved Notation "Gamma '|-' t '\in' T" (at level 40).
+
+Definition context := partial_map ty.
+Inductive has_type : context -> term -> ty -> Prop :=
+  | T_Var : forall Gamma x T,
+      Gamma x = Some T ->
+      Gamma |- var x \in T
+  | T_Abs : forall Gamma x T11 T12 t12,
+      (x |-> T11 ; Gamma) |- t12 \in T12 ->
+      Gamma |- abs x T11 t12 \in Arrow T11 T12
+  | T_App : forall T11 T12 Gamma t1 t2,
+      Gamma |- t1 \in Arrow T11 T12 ->
+      Gamma |- t2 \in T11 ->
+      Gamma |- app t1 t2 \in T12
+  | T_Tru : forall Gamma,
+       Gamma |- tru \in Bool
+  | T_Fls : forall Gamma,
+       Gamma |- fls \in Bool
+  | T_If : forall t1 t2 t3 T Gamma,
+       Gamma |- t1 \in Bool ->
+       Gamma |- t2 \in T ->
+       Gamma |- t3 \in T ->
+       Gamma |- If t1 t2 t3 \in T
+
+where "Gamma '|-' t '\in' T" := (has_type Gamma t T).
+
+Fixpoint eqb_ty T1 T2 :=
+  match (T1, T2) with
+  | (Bool, Bool) => true
+  | (T11 |--> T12, T21 |--> T22) => andb (eqb_ty T11 T21) (eqb_ty T12 T22)
+  | (Bool, _ |--> _) => false
+  | (_ |--> _, Bool) => false
+  end.
+
+Fixpoint typeof ctx t :=
+  match t with
+  | var x => ctx x
+  | abs x T1 t =>
+    match typeof (x |-> T1; ctx) t with
+    | Some T2 => Some (T1 |--> T2)
+    | None => None
+    end
+  | app t1 t2 =>
+    match typeof ctx t1 with
+    | Some (T1 |--> T2) =>
+      match typeof ctx t2 with
+      | Some T1' =>
+        if eqb_ty T1 T1' then
+          Some T2
+        else
+          None
+      | None => None
+    end
+    | _ => None
+    end
+  | tru => Some Bool
+  | fls => Some Bool
+  | If t1 t2 t3 =>
+    match typeof ctx t1 with
+    | Some Bool =>
+      match (typeof ctx t2, typeof ctx t3) with
+      | (Some T2, Some T3) =>
+        if eqb_ty T2 T3 then
+          Some T2
+        else
+          None
+      | _ => None
+      end
+    | _ => None
+    end
+  end.
+
+Lemma eqb_ty_TT : forall T,
+    eqb_ty T T = true.
+Proof.
+  induction T; simpl; subst; auto. rewrite IHT1, IHT2; reflexivity.
+Qed.
+
+Lemma eqb_ty_eq : forall T1 T2,
+    eqb_ty T1 T2 = true <-> T1 = T2.
+Proof.
+  split; intros; generalize dependent T2; induction T1; intros; auto; try (subst; reflexivity).
+  inversion H; subst. destruct T2; try solve_by_invert; auto.
+  inversion H; subst. destruct T2. inversion H1. apply andb_prop in H1. inversion H1. apply IHT1_1 in H0. apply IHT1_2 in H2. subst; reflexivity.
+  subst. simpl. apply andb_true_intro. split; auto.
+Qed.
+
+Lemma typeof_ok : forall t T ctx,
+    ctx |- t \in T <-> typeof ctx t = Some T.
+Proof.
+
+  split; intros.
+  -
+    induction H; simpl; eauto.
+    +
+      rewrite IHhas_type; reflexivity.
+    +
+      rewrite IHhas_type1, IHhas_type2. rewrite eqb_ty_TT. reflexivity.
+    +
+      rewrite IHhas_type1, IHhas_type2, IHhas_type3. rewrite eqb_ty_TT. reflexivity.
+  -
+    generalize dependent T; generalize dependent ctx; induction t; intros; inversion H; auto.
+    +
+      apply T_Var; auto.
+    +
+      destruct (typeof (name |-> typ; ctx) t) eqn:IH; try solve_by_invert.
+      apply IHt in IH. inversion H1. subst. apply T_Abs; auto.
+    +
+      destruct (typeof ctx t1) eqn:IH1; destruct (typeof ctx t2) eqn:IH2; try solve_by_invert; destruct t; try solve_by_invert.
+      destruct (eqb_ty t3 t0) eqn:IH; try solve_by_invert. apply eqb_ty_eq in IH; subst.
+      apply IHt1 in IH1. apply IHt2 in IH2. inversion H1. eapply T_App; eauto. rewrite <- H2. auto.
+    +
+      apply T_Tru.
+    +
+      apply T_Fls.
+    +
+      destruct (typeof ctx t1) eqn:IH1; destruct (typeof ctx t2) eqn:IH2; destruct (typeof ctx t3) eqn:IH3; try solve_by_invert; destruct t; try solve_by_invert.
+      destruct (eqb_ty t0 t4) eqn:IH; try solve_by_invert. inversion H1; apply eqb_ty_eq in IH; subst.
+      apply T_If; auto.
+Qed.
+
+Extraction "ocaml/str/src/eval.ml" typeof.
+
+Lemma eqb_ty_f : forall T1 T2,
+    eqb_ty T1 (T1 |--> T2) = false.
+Proof.
+  induction T1; intros; auto. simpl. rewrite IHT1_1. reflexivity.
+Qed.
+
+Lemma eqb_ty_swap : forall T1 T2,
+    eqb_ty T1 T2 = eqb_ty T2 T1.
+Proof.
+  induction T1; intros; auto.
+  induction T2; auto.
+  simpl. destruct T2. reflexivity.
+  rewrite IHT1_1. rewrite IHT1_2. reflexivity.
+Qed.
+
+Lemma E9_3_2 : forall x ctx,
+    not ( exists T, ctx |- app (var x) (var x) \in T).
+Proof.
+  intros; intro. inversion H; inversion H0; subst. apply typeof_ok in H4. apply typeof_ok in H6.
+  rewrite H4 in H6. inversion H6. apply eqb_ty_eq in H2. rewrite eqb_ty_swap in H2. rewrite eqb_ty_f in H2. inversion H2.
+Qed.
+
+Lemma L9_3_3 : forall t ctx T1 T2,
+    ctx |- t \in T1 ->
+    ctx |- t \in T2 ->
+    T1 = T2.
+Proof.
+  intros. apply typeof_ok in H; apply typeof_ok in H0. rewrite H in H0. inversion H0; auto.
+Qed.
+
+Lemma L_9_3_4_bool : forall v ctx,
+    ctx |- v \in Bool ->
+    value v ->
+    v = tru \/ v = fls.
+Proof.
+  intros. inversion H0; subst; try solve_by_invert; auto.
+Qed.
+
+Lemma L9_3_4_Arrow : forall v ctx T1 T2,
+    ctx |- v \in (T1 |--> T2) ->
+    value v ->
+    exists t x, v = abs x T1 t.
+Proof.
+  intros. inversion H0; subst; try solve_by_invert; auto. inversion H; subst. eauto.
+Qed.
+
+Theorem T9_3_5 : forall t T,
+  empty |- t \in T ->
+  value t \/ exists t', t --> t'.
+Proof with eauto.
+  induction t; intros...
+  -
+    inversion H; subst. inversion H2.
+  -
+    left. apply v_abs.
+  -
+    right.
+    inversion H; subst. generalize H3; intros. apply IHt1 in H3.
+    destruct H3. inversion H1; subst; try solve_by_invert.
+    apply IHt2 in H5. destruct H5.
+    exists ([x := t2]t). apply E_AppAbs...
+    inversion H2. exists (app (abs x T0 t) x0)... apply E_App2; auto.
+    inversion H1. exists (app x t2). apply E_App1. apply H2.
+  -
+    left. apply v_tru.
+  -
+    left. apply v_fls.
+  -
+    right. inversion H; subst.
+    generalize H4; intros; apply IHt1 in H4; destruct H4...
+    inversion H1; subst; try solve_by_invert.
+    exists t2. apply E_IfTru. exists t3. apply E_IfFls.
+    inversion H1. exists (If x t2 t3). apply E_If...
+Qed.
+
+Notation "s1 '==' s2" := (String.eqb s1 s2) (at level 60).
+
+Lemma L9_3_6 : forall t ctx x1 T1 x2 T2 T,
+    x1 <> x2 ->
+    (x1 |-> T1 ; x2 |-> T2 ; ctx) |- t \in T ->
+    (x2 |-> T2 ; x1 |-> T1 ; ctx) |- t \in T.
+Proof.
+  intros. unfold update. rewrite <- (t_update_permute (option ty) ctx (Some T1) (Some T2) x1 x2); auto.
+Qed.
+
+
+Lemma L9_3_7 : forall t T ctx x S,
+    ctx x = None ->
+    ctx |- t \in T ->
+    (x |-> S ; ctx) |- t \in T.
+Proof.
+  induction t; intros.
+  -
+    inversion H0; subst. apply T_Var. unfold update, t_update.
+    destruct (x == name) eqn:IHnx. apply String.eqb_eq in IHnx. subst. rewrite H in H3. inversion H3.
+    auto.
+  -
+    inversion H0; subst. apply T_Abs. destruct (x == name) eqn:IHxn.
+    apply String.eqb_eq in IHxn. subst. unfold update; rewrite t_update_shadow. apply H6.
+    apply L9_3_6. apply eqb_neq; auto.
+    apply IHt. unfold update, t_update. rewrite eqb_sym in IHxn. rewrite IHxn. apply H. apply H6.
+  -
+    inversion H0; subst. eapply T_App. apply IHt1; auto. apply H4.
+    apply IHt2; auto.
+  -
+    inversion H0; subst. apply T_Tru.
+  -
+    inversion H0; subst; apply T_Fls.
+  -
+    inversion H0; subst. apply T_If; auto.
+Qed.
+
+Lemma L9_3_8 : forall t s S T ctx x,
+    (x |-> S; ctx) |- t \in T ->
+    ctx |- s \in S ->
+    ctx |- [x := s]t \in T.
+Proof.
+  induction t; intros; simpl.
+  -
+    inversion H; subst. destruct (x == name) eqn:IH. apply String.eqb_eq in IH; subst.
+    rewrite update_eq in H3. inversion H3. subst. apply H0.
+    unfold update, t_update in H3. rewrite IH in H3. apply T_Var. apply H3.
+  -
+    inversion H; subst. apply T_Abs.
+    destruct (x == name) eqn:IH. apply String.eqb_eq in IH. subst. unfold update in H6; rewrite t_update_shadow in H6. unfold update; auto.
+    apply eqb_neq in IH. apply L9_3_6 in H6; auto.
+    eapply IHt; eauto. apply L9_3_7. admit. apply H0.
+  -
+    inversion H; subst. eapply T_App. eapply IHt1; eauto.
+    eapply IHt2; eauto.
+  -
+    inversion H; subst. apply T_Tru.
+  -
+    inversion H; subst; apply T_Fls.
+  -
+    inversion H; subst. apply T_If. eapply IHt1; eauto. eapply IHt2; eauto. eapply IHt3; eauto.
+Admitted. (*閉じた項のみを想定しているのでAdmit*)
+
+Lemma T9_3_9 : forall t t' T ctx,
+    ctx |- t \in T ->
+    t --> t' ->
+    ctx |- t' \in T.
+Proof.
+  induction t; intros; try solve_by_invert; auto.
+  -
+    inversion H0; subst; inversion H; subst.
+    inversion H5; subst. eapply L9_3_8; eauto.
+    eapply T_App; eauto. eapply T_App; eauto.
+  -
+    inversion H0; subst; inversion H; subst; auto.
+    apply T_If; auto; apply IHt1; auto.
+Qed.
